src/circuits/circuit_encoding.lean
@@ -1,5 +1,21 @@
 import circuits.basic
 import polytime.lemmas
 
+open tencodable tree
+open_locale tree complexity_class
 
+variables {α β : Type} [tencodable α] [tencodable β]
+
+def encode_function [fintype α] : tencodable (α → β) :=
+by haveI : decidable_eq α := decidable_eq_of_encodable α; exact 
+tencodable.of_left_injection (λ f, ((finset.univ : finset α).sort lift_le).map (λ x, (⟨x, f x⟩ : Σ _ : α, β)))
+  (λ l, if H : ∀ a, a ∈ l.keys then some (λ x, option.get (list.lookup_is_some.mpr (H x))) else none) 
+  (λ b, begin
+    have : ∀ (a : α) (f : α → β), (((finset.univ : finset α).sort lift_le).map (λ x, (⟨x, f x⟩ : Σ _ : α, β))).lookup a = some (f a),
+    { intros a f, apply list.mem_lookup, { simp [list.nodupkeys, list.keys], }, simp, },
+    rw dif_pos, swap, { simp [← list.lookup_is_some, this], },
+    rw option.some_inj, ext a, simp [this],
+  end)
+
+#check sigma.mk
 
